case_study/RiscvPmp/FemtoKernel.v
@@ -366,10 +366,9 @@ Module inv := invariants.
       asn_pmp_entries (term_list (asn_femto_pmpentries (term_var "a" -ᵇ term_val ty_xlenbits (bv.of_N handler_addr)))) ∗ (* Different handler sizes cause different entries *)
       asn_pmp_addr_access (term_list (asn_femto_pmpentries (term_var "a" -ᵇ term_val ty_xlenbits (bv.of_N handler_addr)))) (term_val ty_privilege User) ∗
       (∃ "oldvalue",  ∃ "s", (
-          term_var "a" +ᵇ term_val ty_xlenbits (bv.of_N mmio_handler_size) ↦ₘ (term_var "oldvalue") ∗
-          (term_unop (uop.bvtake 1) (term_var "oldvalue") = term_var "s") ∗
-          asn_mmio_state_pred (term_var "s") 
-          (* asn.formula (formula_user (mmio_state_prot bytes_per_word) [term_var "oldvalue"; term_var "s"; term_var "s'"]) *)
+          term_var "a" +ᵇ term_val ty_xlenbits (bv.of_N mmio_handler_size) ↦ₘ (term_var "oldvalue")
+          ∗ (term_unop (uop.bvtake 1) (term_var "oldvalue") = term_var "s")
+          ∗ asn_mmio_state_pred (term_var "s")
       ))
       ∗ asn_mmio_trace_state_inv.
 
@@ -497,7 +496,7 @@ Import Erasure.notations.
   End FemtoKernel.
 
   (* Avoid expanding interp_ptstomem when doing simplifications *)
-  Arguments interp_ptstomem : simpl never. 
+  Arguments interp_ptstomem : simpl never.
 
   Definition advAddrs : list (bv xlenbits) := bv.seqBv (bv.of_N adv_addr) (adv_addr_end - adv_addr).
 
@@ -792,7 +791,7 @@ Import Erasure.notations.
     iDestruct "Hbase" as "(Hpre & Hpc & Hnextpc)".
     iDestruct "Hpre" as "( [%Ha _] & [#Haoffset _] & Hmstatus & Hmip & Hmie & Hmtvec & Hmcause & [%Hmepcv Hmepc] & Hpts & Hcurpriv & Hpmpentries & HaccU & Hpred)".
     iApply (femto_handler_verified_block1 with "[Hmstatus Hmtvec Hmcause Hmip Hmie Hmepc Hpts Hcurpriv Hpmpentries Hpc Hnextpc Hinstrs1 HaccU Hpred]").
-    - iFrame "Hmstatus Hmtvec Hmcause Hmip Hmie Hmepc Hpts Hcurpriv Haoffset Hpred". iFrame "Hpc Hnextpc HaccU". 
+    - iFrame "Hmstatus Hmtvec Hmcause Hmip Hmie Hmepc Hpts Hcurpriv Haoffset Hpred". iFrame "Hpc Hnextpc HaccU".
       iSplitL "Hpmpentries".
       -- cbn; repeat iSplit; auto.
       -- cbv in Ha. subst. iFrame "Hinstrs1".
@@ -808,7 +807,7 @@ Import Erasure.notations.
       cbn in Ha, Ha2, Han. subst.
       iSplitR "Hinstrs Hinstrs0 Hinstrs1 Hinstrs2".
       + iFrame "Hpmpentries Hmem HaccU". cbn. iFrame. repeat iSplitL "". auto. auto. auto. auto.
-        iDestruct "Hstate" as "[Hstate Hprot]". iFrame. iDestruct "Hprot" as (v0) "[%Hprot _]". iExists v0. iPureIntro. split; auto. 
+        iDestruct "Hstate" as "[Hstate Hprot]". iFrame.
       + iFrame "Hinstrs Hinstrs0 Hinstrs1 Hinstrs2".
  Qed.
 
@@ -830,7 +829,7 @@ Import Erasure.notations.
     }
     iIntros "%an (Hpc & [%v Hnextpc] & Hinstrs0 & Hpost0)".
     iDestruct "Hpost0" as "(_ & _ & Hmstatus & Hmie & Hmip & Hscratch & Hmtvec & Hmcause & Hmepc & Hpts & Hcurpriv & Hpmpentries & HaccU & Hpred)".
-    iDestruct "Hpred" as "((%vold & %vnew & %s & %s' & Hx5 & Hold & Hstate & [%Hpold _] & Hpred ) & Hinv)".
+    iDestruct "Hpred" as "((%vold & %vnew & %s & %s' & Hx5 & Hold & [Hpold _] & Hstate & Hpred ) & Hinv)".
     (* Tut: We destruct over the two cases even / odd number in t0 *)
     iDestruct "Hpred" as "[HpredL | HpredR]".
     - (* Tut: Case legal value i.e. we do not jump and therefore enter block1 *)
@@ -838,11 +837,11 @@ Import Erasure.notations.
       + iModIntro. iIntros "IH". iApply "Hind". iFrame "IH".
       + iFrame "Hnextpc Hpc Hmstatus Hmip Hmie Hscratch Hmtvec Hmcause Hmepc Hx5 Hpts Hcurpriv".
         iSplitR "Hinstrs Hinstrs0 Hinstrs1 Hinstrs2".
-        ++ iDestruct "Hinv" as "#Hinv". iDestruct "HpredL" as "[(%s_prot & Hprot & _) [%Han _]]". cbn in *.
+        ++ iDestruct "Hinv" as "#Hinv". iDestruct "HpredL" as "([%s_prot _] & [Hprot _] & [%Han _])". cbn in *.
            subst.
            iSplitL ""; auto. iSplitL ""; auto.
            iFrame "Hpmpentries HaccU".
-           iSplitL "Hold Hstate Hprot"; auto. iExists vold. iExists s, s'. iFrame "Hold". iSplit; auto.
+           iSplitL "Hold Hstate Hprot"; auto. iExists vold. iExists s. iFrame "Hold". iSplit; auto. iSplit; auto. admit.
         ++ subst. iFrame "Hinstrs Hinstrs0 Hinstrs1 Hinstrs2".
     - (* Tut: Case illegal value i.e. we jump and therefore enter block2 *)
       iApply (femtokernel_handler_safe_block2 with "[]").
@@ -854,9 +853,9 @@ Import Erasure.notations.
               iSplitL ""; auto. iSplitL ""; auto.
               iFrame "Hpmpentries HaccU".
               iSplitL "Hold Hstate"; auto.
-              iExists vold. iExists s. iExists s'. iFrame "Hold Hstate". auto.
+              iExists vold. iExists s. iFrame "Hold Hstate".
         ++ subst. iFrame "Hinstrs Hinstrs0 Hinstrs1 Hinstrs2".
-Qed.
+Admitted.
 
 
   (* TODO: this lemma feels very incremental wrt to the last one; merge? *)
@@ -1227,4 +1226,3 @@ Qed.
 (* Local Variables: *)
 (* proof-omit-proofs-option: t *)
 (* End: *)
-
